test/monniaux/builtins/fma.c
@@ -1,0 +1,12 @@
+#include <math.h>
+#include <stdio.h>
+#include <stdlib.h>
+
+int main(int argc, char **argv) {
+  if (argc < 4) return 1;
+  double x = strtod(argv[1], NULL);
+  double y = strtod(argv[2], NULL);
+  double z = strtod(argv[3], NULL);
+  printf("%g %g %g\n", __builtin_fma(x, y, z), fma(x, y, z), x*y + z);
+  return 0;
+}
